commit

AP/AP/HistBlind/A.lean
@@ -1,4 +1,4 @@
-import AP.AP.Determinacy
+import AP.AP.HistBlind.Basic
 
 namespace AP
 
@@ -45,42 +45,19 @@ theorem State.chooseDMove_setHist {s : State} {hist} :
 (s.setHist hist).chooseDMove = s.chooseDMove := by
   simp [chooseDMove]
 
-def AStrat.histBlind (a : AStrat) : Prop :=
-  ∀ s hist, AState s → sys.WF (s.setHist hist) →
-  sys.hasTr s → a.f (s.setHist hist) = a.f s
-
-def DStrat.histBlind (d : DStrat) : Prop :=
-  ∀ s hist, DState s → sys.WF (s.setHist hist) →
-  sys.hasTr s → d.f (s.setHist hist) = d.f s
-
 open Classical in noncomputable
 def aHistBlind : AStrat := .mk' # λ s => do
   let s' ← choose? # λ (s' : State) => sys.WF s' ∧ s'.setHist s.hist = s
   let a ← choose? # λ (a : AStrat) => a.WF ∧ ∀ (d : DStrat), d.WF → s'.a_wins ⟨a, d⟩
   return a.f s'
 
-open Classical in noncomputable
-def dHistBlind : DStrat := .mk' # λ s => do
-  let s' ← choose? # λ (s' : State) => sys.WF s' ∧ s'.setHist s.hist = s
-  let d ← choose? # λ (d : DStrat) => d.WF ∧ ∀ (a : AStrat), a.WF → s'.d_wins ⟨a, d⟩
-  return d.f s'
-
 instance : aHistBlind.WF := by unfold aHistBlind; infer_instance
-instance : dHistBlind.WF := by unfold dHistBlind; infer_instance
 
 @[simp] theorem histBlind_aHistBlind : aHistBlind.histBlind := by
   intro s hist hs hs' h₁; unfold aHistBlind
   have h₃ : (λ s' => sys.WF s' ∧ s'.setHist hist = s.setHist hist) =
     (λ s' => sys.WF s' ∧ s'.setHist s.hist = s); simp [State.ext_iff]
   simp [AStrat.mk', Option.pure_def, Option.bind_eq_bind, AStrat.f_mk,
-    mk_strat_fn, choose?_eq_ite, h₃]
-  split_ifs with h₂ <;> first | (rw [h₃] at h₂; contradiction) | simp
-
-@[simp] theorem histBlind_dHistBlind : dHistBlind.histBlind := by
-  intro s hist hs hs' h₁; unfold dHistBlind
-  have h₃ : (λ s' => sys.WF s' ∧ s'.setHist hist = s.setHist hist) =
-    (λ s' => sys.WF s' ∧ s'.setHist s.hist = s); simp [State.ext_iff]
-  simp [DStrat.mk', Option.pure_def, Option.bind_eq_bind, DStrat.f_mk,
     mk_strat_fn, choose?_eq_ite, h₃]
   split_ifs with h₂ <;> first | (rw [h₃] at h₂; contradiction) | simp
 
@@ -411,117 +388,6 @@ theorem State.a_hws_histBlind_of_a_hws {s} [hs : sys.WF s] (h : s.a_hws) :
   rw [DState.a_hws_iff_tr] at h₁
   apply h₁; exact h₂
 
-theorem State.d_hws_histBlind_of_d_hws {s} [hs : sys.WF s] (h : s.d_hws) :
-∃ (d : DStrat), d.WF ∧ d.histBlind ∧ ∀ (a : AStrat), a.WF → s.d_wins ⟨a, d⟩ := by
-  sorry
-
-#check 0 #exit
-
-  contrapose h
-  push_neg at h
-  simp at h ⊢
-  apply a_hws_of_ind (p := λ s => ∀ (d : DStrat), d.WF → d.histBlind →
-    ∃ a, a.WF ∧ s.a_wins ⟨a, d⟩) h <;> clear! s
-  · intro sa ha ih
-    obtain ⟨a, Ha, h₁⟩ := ih dHistBlind inferInstance (by simp)
-    obtain ⟨sd, h₂⟩ := a.validTr # ha.hasTr_of_a_wins h₁
-    generalize a.f sa = pa at h₂
-    use pa, sd, h₂
-    intro d Hd h₃
-    specialize ih d Hd h₃
-    clear! a h₃
-    obtain ⟨a, Ha, ih⟩ := ih
-  intro sd hd pd sa ih h₁ n
-  specialize ih # n + 1
-  simp at ih; split at ih; simp at ih; nm x sa' h₂; clear x
-  simp [-DState.tr_eq_some_iff, dHistBlind, mk_strat_fn] at h₂
-  have h₃ : ∃ s', sys.WF s' ∧ s'.setHist sd.hist = sd
-  · use sd; simp; infer_instance
-  generalize hd' : Classical.epsilon (λ s' => sys.WF s' ∧ s'.setHist sd.hist = sd) = sd'
-  have h₄ := Classical.epsilon_spec h₃ <;> rw [hd'] at h₄
-  rcases h₄ with ⟨h₄, h₅⟩
-  have h₆ : ∃ (d : DStrat), d.WF ∧ ∀ (a : AStrat), a.WF → sd'.d_wins ⟨a, d⟩
-  · sorry
-  generalize h₇ : Classical.epsilon (λ (d : DStrat) => d.WF ∧ ∀ (a : AStrat), a.WF →
-    sd'.d_wins ⟨a, d⟩) = d
-  have h₈ := Classical.epsilon_spec h₆; rw [h₇] at h₈
-  rcases h₈ with ⟨h₈, h₉⟩
-  have h₅' := setHist_eq_comm.mp h₅
-  have hd₁ : DState sd'; use h₄; rw [←h₅']; simp
-  have H₁ : sys.validTr sd (d.f sd'); rw [←h₅]; simp
-  simp [-DState.tr_eq_some_iff, choose?_eq_ite, h₃, hd', h₆, h₇, H₁] at h₂
-  clear H₁
-  
-  rw [←h₅] at h₂
-  simp [-DState.tr_eq_some_iff] at h₂
-  rcases h₂ with ⟨sa₁, ha₁, rfl⟩
-
-#check 0 #exit
-
-  use dHistBlind, inferInstance, by simp
-  contrapose h
-  push_neg at h
-  simp at h ⊢
-  apply a_hws_of_ind (p := λ s => ∃ (a : AStrat), a.WF ∧
-    s.a_wins ⟨a, dHistBlind⟩) h <;> clear! s
-  · rintro sa ha ⟨a, Ha, ih⟩
-    obtain ⟨sd, h₁⟩ := ha.validTr_of_a_wins ih
-    dsimp at h₁
-    use a.f sa, sd, h₁, a, Ha
-    intro n
-    specialize ih # n + 1
-    simp [h₁] at ih
-    exact ih
-  intro sd hd pd sa ih h₁
-  specialize ih # n + 1
-  simp at ih; split at ih; simp at ih; nm x sa' h₂; clear x
-  simp [-DState.tr_eq_some_iff, dHistBlind, mk_strat_fn] at h₂
-  have h₃ : ∃ s', sys.WF s' ∧ s'.setHist sd.hist = sd
-  · use sd; simp; infer_instance
-  generalize hd' : Classical.epsilon (λ s' => sys.WF s' ∧ s'.setHist sd.hist = sd) = sd'
-  have h₄ := Classical.epsilon_spec h₃ <;> rw [hd'] at h₄
-  rcases h₄ with ⟨h₄, h₅⟩
-  have h₆ : ∃ (d : DStrat), d.WF ∧ ∀ (a : AStrat), a.WF → sd'.d_wins ⟨a, d⟩
-  · sorry
-  generalize h₇ : Classical.epsilon (λ (d : DStrat) => d.WF ∧ ∀ (a : AStrat), a.WF →
-    sd'.d_wins ⟨a, d⟩) = d
-  have h₈ := Classical.epsilon_spec h₆; rw [h₇] at h₈
-  rcases h₈ with ⟨h₈, h₉⟩
-  have h₅' := setHist_eq_comm.mp h₅
-  have hd₁ : DState sd'; use h₄; rw [←h₅']; simp
-  have H₁ : sys.validTr sd (d.f sd'); rw [←h₅]; simp
-  simp [-DState.tr_eq_some_iff, choose?_eq_ite, h₃, hd', h₆, h₇, H₁] at h₂
-  clear H₁
-  
-  rw [←h₅] at h₂
-  simp [-DState.tr_eq_some_iff] at h₂
-
-#check 0 #exit
-
-  contrapose h
-  push_neg at h
-  simp at h ⊢
-  apply a_hws_of_ind (p := λ s => ∀ (d : DStrat), d.WF → d.histBlind →
-    ∃ a, a.WF ∧ s.a_wins ⟨a, d⟩) h <;> clear! s
-  rotate_left
-  · intro sd hd pd sa ih h₁ d Hd h₂
-    sorry
-  · intro sa ha ih
-    have h₁ := ih dHistBlind inferInstance (by simp)
-    obtain ⟨a, Ha, h₁⟩ := h₁
-    obtain ⟨sd, hd⟩ := ha.validTr_of_a_wins h₁
-    dsimp at hd
-    use a.f sa, sd, hd
-    intro d Hd h₂
-    specialize ih d Hd h₂
-    sorry
-
-#check 0 #exit
-
 theorem State.a_hws_iff_a_hws_histBlind {s} [hs : sys.WF s] : s.a_hws ↔
 ∃ (a : AStrat), a.WF ∧ a.histBlind ∧ ∀ (d : DStrat), d.WF → s.a_wins ⟨a, d⟩ :=
   ⟨a_hws_histBlind_of_a_hws, λ ⟨a, Ha, h₁, h₂⟩ => by use a⟩
-
-theorem State.d_hws_iff_d_hws_histBlind {s} [hs : sys.WF s] : s.d_hws ↔
-∃ (d : DStrat), d.WF ∧ d.histBlind ∧ ∀ (a : AStrat), a.WF → s.d_wins ⟨a, d⟩ :=
-  ⟨d_hws_histBlind_of_d_hws, λ ⟨d, Hd, h₁, h₂⟩ => by use d⟩
