AP/AP/HistBlind/D.lean
@@ -1,0 +1,13 @@
+import AP.AP.HistBlind.A
+
+namespace AP
+
+theorem State.d_hws_histBlind_of_d_hws {s} [hs : sys.WF s] (h : s.d_hws) :
+∃ (d : DStrat), d.WF ∧ d.histBlind ∧ ∀ (a : AStrat), a.WF → s.d_wins ⟨a, d⟩ := by
+  sorry
+
+#check 0 #exit
+
+theorem State.d_hws_iff_d_hws_histBlind {s} [hs : sys.WF s] : s.d_hws ↔
+∃ (d : DStrat), d.WF ∧ d.histBlind ∧ ∀ (a : AStrat), a.WF → s.d_wins ⟨a, d⟩ :=
+  ⟨d_hws_histBlind_of_d_hws, λ ⟨d, Hd, h₁, h₂⟩ => by use d⟩
