AP/AP/HistBlind/Defs.lean
@@ -1,0 +1,11 @@
+import AP.AP.Determinacy
+
+namespace AP
+
+def AStrat.histBlind (a : AStrat) : Prop :=
+  ∀ s hist, AState s → sys.WF (s.setHist hist) →
+  sys.hasTr s → a.f (s.setHist hist) = a.f s
+
+def DStrat.histBlind (d : DStrat) : Prop :=
+  ∀ s hist, DState s → sys.WF (s.setHist hist) →
+  sys.hasTr s → d.f (s.setHist hist) = d.f s
